HybridVerifVecs/hs_vc_spartan.thy
@@ -1,0 +1,200 @@
+theory hs_vc_spartan
+  imports hs_prelims_dyn_sys
+                        
+begin
+
+
+chapter \<open>Hybrid System Verification\<close>
+
+type_synonym 'a pred = "'a \<Rightarrow> bool"
+
+no_notation Transitive_Closure.rtrancl ("(_\<^sup>*)" [1000] 999)
+
+notation Union ("\<mu>")
+
+definition fbox :: "('a \<Rightarrow> 'b set) \<Rightarrow> 'b pred \<Rightarrow> 'a pred"
+  where "fbox F P = (\<lambda>s. (\<forall>s'. s' \<in> F s \<longrightarrow> P s'))"
+
+section \<open>Verification of regular programs\<close>
+
+text \<open>First we add lemmas for computation of weakest liberal preconditions (wlps).\<close>
+
+lemma fbox_eta[simp]: "fbox (\<lambda>s. {s}) P = P"
+  unfolding fbox_def by simp
+
+lemma fbox_iso: "P \<le> Q \<Longrightarrow> fbox F P \<le> fbox F Q"
+  unfolding fbox_def by auto
+
+lemma fbox_def_univD: "fbox F P s = True \<Longrightarrow> (\<forall>s'. s' \<in> (F s) \<longrightarrow> P s')"
+  unfolding fbox_def by auto
+
+lemma fbox_invariants: 
+  assumes "I \<le> fbox F I" and "J \<le> fbox F J"
+  shows "(\<lambda>s. I s \<and> J s) \<le> fbox F (\<lambda>s. I s \<and> J s)"
+    and "(\<lambda>s. I s \<or> J s) \<le> fbox F (\<lambda>s. I s \<or> J s)"
+  using assms unfolding fbox_def by auto
+
+text \<open>Next, we introduce assignments and their wlps.\<close>
+
+definition vec_upd :: "('a^'n) \<Rightarrow> 'n \<Rightarrow> 'a \<Rightarrow> 'a^'n"
+  where "vec_upd s i a \<equiv> \<chi> j. ((($) s)(i := a)) j"
+
+definition assign :: "'n \<Rightarrow> ('a^'n \<Rightarrow> 'a) \<Rightarrow> ('a^'n) \<Rightarrow> ('a^'n) set" ("(2_ ::= _)" [70, 65] 61) 
+  where "(x ::= e) \<equiv> (\<lambda>s. {vec_upd s x (e s)})" 
+
+lemma fbox_assign[simp]: "fbox (x ::= e) Q = (\<lambda>s. Q (\<chi> j. ((($) s)(x := (e s))) j))"
+  unfolding vec_upd_def assign_def by (subst fbox_def) simp
+
+text \<open>The wlp of a (kleisli) composition is just the composition of the wlps.\<close>
+
+definition kcomp :: "('a \<Rightarrow> 'b set) \<Rightarrow> ('b \<Rightarrow> 'c set) \<Rightarrow> ('a  \<Rightarrow> 'c set)" (infixl ";" 75) where
+  "F ; G = \<mu> \<circ> \<P> G \<circ> F"
+
+lemma kcomp_eq: "(f ; g) x = \<Union> {g y |y. y \<in> f x}"
+  unfolding kcomp_def image_def by auto
+
+lemma fbox_kcomp: "fbox (G ; F) P = fbox G (fbox F P)"
+  unfolding fbox_def kcomp_def by auto
+
+lemma fbox_kcomp_ge:
+  assumes "P \<le> fbox F R" "R \<le> fbox G Q"
+  shows "P \<le> fbox (F ; G) Q"
+  apply(subst fbox_kcomp) 
+  by (rule order.trans[OF assms(1)]) (rule fbox_iso[OF assms(2)])
+
+text \<open>We also have an implementation of the conditional operator and its wlp.\<close>
+
+definition ifthenelse :: "'a pred \<Rightarrow> ('a \<Rightarrow> 'b set) \<Rightarrow> ('a \<Rightarrow> 'b set) \<Rightarrow> ('a \<Rightarrow> 'b set)"
+  ("IF _ THEN _ ELSE _ FI" [64,64,64] 63) where 
+  "IF P THEN X ELSE Y FI \<equiv> (\<lambda>s. if P s then X s else Y s)"
+
+lemma fbox_if_then_else:
+  "fbox (IF T THEN X ELSE Y FI) Q = (\<lambda>s. (T s \<longrightarrow> fbox X Q s) \<and> (\<not> T s \<longrightarrow> fbox Y Q s))"
+  unfolding fbox_def ifthenelse_def by auto
+
+lemma fbox_if_then_else_ge:
+  assumes "(\<lambda>s. P s \<and> T s) \<le> fbox X Q"
+    and "(\<lambda>s. P s \<and> \<not> T s) \<le> fbox Y Q"
+  shows "P \<le> fbox (IF T THEN X ELSE Y FI) Q"
+  using assms unfolding fbox_def ifthenelse_def by auto
+
+lemma fbox_if_then_elseI:
+  assumes "T s \<longrightarrow> fbox X Q s"
+    and "\<not> T s \<longrightarrow> fbox Y Q s"
+  shows "fbox (IF T THEN X ELSE Y FI) Q s"
+  using assms unfolding fbox_def ifthenelse_def by auto
+
+text \<open>The final wlp we add is that of the finite iteration.\<close>
+
+abbreviation "skip \<equiv> (\<lambda>s. {s})"
+
+definition kpower :: "('a \<Rightarrow> 'a set) \<Rightarrow> nat \<Rightarrow> ('a \<Rightarrow> 'a set)" 
+  where "kpower f n = (\<lambda>s. ((;) f ^^ n) skip s)"
+
+lemma kpower_base:
+  shows "kpower f 0 s = {s}"
+    and "kpower f (Suc 0) s = f s"
+  unfolding kpower_def by(auto simp: kcomp_eq)
+
+lemma kpower_simp: "kpower f (Suc n) s = (f ; kpower f n) s"
+  unfolding kcomp_eq apply(induct n)
+  unfolding kpower_base apply(rule subset_antisym, clarsimp, force, clarsimp)
+  unfolding kpower_def kcomp_eq by simp
+
+definition kleene_star :: "('a \<Rightarrow> 'a set) \<Rightarrow> ('a \<Rightarrow> 'a set)" ("(_\<^sup>*)" [1000] 999)
+  where "(f\<^sup>*) s = \<Union> {kpower f n s |n. n \<in> UNIV}"
+
+lemma kpower_inv: 
+  fixes F :: "'a \<Rightarrow> 'a set"
+  assumes "\<forall>s. I s \<longrightarrow> (\<forall>s'. s' \<in> F s \<longrightarrow> I s')" 
+  shows "\<forall>s. I s \<longrightarrow> (\<forall>s'. s' \<in> (kpower F n s) \<longrightarrow> I s')"
+  apply(clarsimp, induct n)
+  unfolding kpower_base apply simp
+  unfolding kpower_simp apply(simp add: kcomp_eq, clarsimp) 
+  apply(subgoal_tac "I y", simp)
+  using assms by blast
+
+lemma kstar_inv: "I \<le> fbox F I \<Longrightarrow> I \<le> fbox (F\<^sup>*) I"
+  unfolding kleene_star_def fbox_def apply clarsimp
+  apply(unfold le_fun_def, subgoal_tac "\<forall>x. I x \<longrightarrow> (\<forall>s'. s' \<in> F x \<longrightarrow> I s')")
+  apply(thin_tac "\<forall>x. I x \<le> (\<forall>s'. s' \<in> F x \<longrightarrow> I s')")
+  using kpower_inv[of I F] by blast simp
+
+lemma fbox_kstarI:
+  assumes "P \<le> I" and "I \<le> Q" and "I \<le> fbox F I" 
+  shows "P \<le> fbox (F\<^sup>*) Q"
+proof-
+  have "I \<le> fbox (F\<^sup>*) I"
+    using assms(3) kstar_inv by blast
+  hence "P \<le> fbox (F\<^sup>*) I"
+    using assms(1) by auto
+  also have "fbox (F\<^sup>*) I \<le> fbox (F\<^sup>*) Q"
+    by (rule fbox_iso[OF assms(2)])
+  finally show ?thesis .
+qed
+
+
+section \<open>Verification of hybrid programs\<close>
+
+notation g_orbital ("(1x\<acute>=_ & _ on _ _ @ _)")
+
+abbreviation g_evol ::"(('a::banach)\<Rightarrow>'a) \<Rightarrow> 'a pred \<Rightarrow> 'a \<Rightarrow> 'a set" 
+  ("(1x\<acute>=_ & _)") where "(x\<acute>=f & G) s \<equiv> (x\<acute>=f & G on UNIV UNIV @ 0) s"
+
+
+subsection \<open>Verification by providing solutions\<close>
+
+lemma fbox_g_orbital: "fbox (x\<acute>=f & G on T S @ t\<^sub>0) Q = 
+  (\<lambda>s. \<forall>X\<in>ivp_sols (\<lambda>t. f) T S t\<^sub>0 s. \<forall>t\<in>T. (\<forall>\<tau>\<in>down T t. G (X \<tau>)) \<longrightarrow> Q (X t))"
+  unfolding fbox_def g_orbital_eq by (auto simp: fun_eq_iff)
+
+context local_flow
+begin
+
+lemma fbox_g_orbit: "fbox (x\<acute>=f & G on T S @ 0) Q = 
+  (\<lambda>s. s \<in> S \<longrightarrow> (\<forall>t\<in>T. (\<forall>\<tau>\<in>down T t. G (\<phi> \<tau> s)) \<longrightarrow> Q (\<phi> t s)))" (is "_ = ?wlp")
+  unfolding fbox_g_orbital apply(rule ext, safe, clarsimp)
+    apply(erule_tac x="\<lambda>t. \<phi> t s" in ballE)
+  using in_ivp_sols apply(force, force, force simp: init_time ivp_sols_def)
+  apply(subgoal_tac "\<forall>\<tau>\<in>down T t. X \<tau> = \<phi> \<tau> s", simp_all, clarsimp)
+  apply(subst eq_solution, simp_all add: ivp_sols_def)
+  using init_time by auto
+
+lemma fbox_g_orbit_ivl: "t \<ge> 0 \<Longrightarrow> t \<in> T \<Longrightarrow> fbox (x\<acute>=f & G on {0..t} S @ 0) Q = 
+  (\<lambda>s. s \<in> S \<longrightarrow> (\<forall>t\<in>{0..t}. (\<forall>\<tau>\<in>{0..t}. G (\<phi> \<tau> s)) \<longrightarrow> Q (\<phi> t s)))"
+  unfolding fbox_g_orbital apply(rule ext, clarsimp, safe)
+    apply(erule_tac x="\<lambda>t. \<phi> t s" in ballE, force)
+  using in_ivp_sols_ivl apply(force simp: closed_segment_eq_real_ivl)
+  using in_ivp_sols_ivl apply(force simp: ivp_sols_def)
+   apply(subgoal_tac "\<forall>t\<in>{0..t}. (\<forall>\<tau>\<in>{0..t}. X \<tau> = \<phi> \<tau> s)", simp, clarsimp)
+  apply(subst eq_solution_ivl, simp_all add: ivp_sols_def)
+     apply(rule has_vderiv_on_subset, force, force simp: closed_segment_eq_real_ivl)
+    apply(force simp: closed_segment_eq_real_ivl)
+  using interval_time init_time apply (meson is_interval_1 order_trans) 
+  using init_time by force
+
+lemma fbox_orbit: "fbox \<gamma>\<^sup>\<phi> Q = (\<lambda>s. s \<in> S \<longrightarrow> (\<forall> t \<in> T. Q (\<phi> t s)))"
+  unfolding orbit_def fbox_g_orbit by simp
+
+end
+
+
+subsection\<open> Verification with differential invariants \<close>
+
+lemma fbox_g_orbital_guard: 
+  assumes "H = (\<lambda>s. G s \<and> Q s)"
+  shows "fbox (x\<acute>=f & G on T S @ t\<^sub>0) H = fbox (x\<acute>=f & G on T S @ t\<^sub>0) Q"
+  unfolding fbox_g_orbital using assms by auto
+
+lemma fbox_g_orbital_inv:
+  assumes "P \<le> I" and "I \<le> fbox (x\<acute>=f & G on T S @ t\<^sub>0) I" and "I \<le> Q"
+  shows "P \<le> fbox (x\<acute>=f & G on T S @ t\<^sub>0) Q"
+  using assms(1) apply(rule order.trans)
+  using assms(2) apply(rule order.trans)
+  by (rule fbox_iso[OF assms(3)])
+
+lemma fbox_diff_inv: 
+  "(I \<le> fbox (x\<acute>=f & G on T S @ t\<^sub>0) I) = diff_invariant I f T S t\<^sub>0 G"
+  by (auto simp: diff_invariant_def ivp_sols_def fbox_def g_orbital_eq)
+
+end
